fin is better, but lemma is wrong :(

lib/SystemF.v
@@ -1,151 +1,17 @@
 Require Export Lambda.Util.
 From Equations Require Export Equations.
+Require Coq.Vectors.Fin.
+Module FIN.
+  Export Coq.Vectors.Fin.
+
+  Derive Signature for t.
+  Equations Derive NoConfusion NoConfusionHom Subterm for t.
+End FIN.
 
 (** * System F *)
 
-Equations len {A : Set} : list A -> nat :=
-| []    => 0
-| _ :: l => S (len l).
-
-Reserved Notation "x '≤' y" (at level 80, no associativity).
-
-Inductive LE (n : nat) : nat -> Set :=
-| LE_n : n ≤ n
-| LE_S m :
-  n ≤ m ->
-  n ≤ S m
-where "x ≤ y" := (LE x y) : type_scope.
-
-Equations Derive NoConfusion NoConfusionHom Subterm for nat.
-
-Derive Signature for LE.
-Equations Derive NoConfusion for LE.
-
-Equations S_LE : forall {n m}, n ≤ m -> S n ≤ S m :=
-  S_LE (LE_n n) := LE_n (S n);
-  S_LE (LE_S _ _ hnm) := LE_S _ _ (S_LE hnm).
-
-Equations LE_0_l : forall n : nat, 0 ≤ n :=
-  LE_0_l 0     := LE_n _;
-  LE_0_l (S n) := LE_S _ _ (LE_0_l n).
-
-Definition bruh (n m : nat) (ρ : forall r, r ≤ m -> r ≤ n) : m ≤ n := ρ m (LE_n m).
-
-Equations S_impl_LE : forall {n m}, S n ≤ S m -> n ≤ m :=
-  S_impl_LE (LE_n (S n)) := LE_n n;
-  S_impl_LE (LE_S n (S m) h) := LE_S _ _ (S_impl_LE h).
-
-Lemma not_S_n_LE_n : forall (n : nat), S n ≤ n -> Empty_set.
-Proof.
-  intros n h; induction n as [| n ih].
-  - inv h.
-  - apply S_impl_LE,ih in h.
-    apply h.
-Defined.
-
-Lemma LE_n_eq : forall {n : nat} (h : n ≤ n), h = LE_n n.
-Proof.
-  intros n h; depelim h.
-  - inv H. apply inj_right_pair in H1; subst. reflexivity.
-  - exfalso. apply not_S_n_LE_n in h. inv h.
-Defined.
-
-Equations Derive NoConfusionHom for LE.
-Next Obligation.
-  unfold NoConfusionHom_LE in H.
-  depelim a; depelim b; cbn in *; subst; try contradiction.
-  - rewrite LE_n_eq; reflexivity.
-  - reflexivity.
-Defined.
-Next Obligation.
-  unfold noConfusionHom_LE_obligation_2,
-    noConfusionHom_LE_obligation_1.
-  unfold NoConfusionHom_LE in *.
-  depelim a; depelim b; cbn in *; subst; try contradiction.
-  - pose proof LE_n_eq b0 as b0eq; subst.
-    unfold eq_ind_r,eq_ind, eq_sym,LE_n_eq.
-    unfold eq_ind_r,eq_ind,eq_sym,inj_right_pair,f_equal.
-    rewrite eq_dec_refl.
-    unfold K_dec.
-    rewrite <- Eqdep_dec.eq_rect_eq_dec.
-    + depelim e; reflexivity.
-    + intros x y. left.
-      rewrite Eqdep_dec.UIP_refl_nat with (x := x).
-      rewrite Eqdep_dec.UIP_refl_nat with (x := y).
-      reflexivity.
-  - unfold eq_ind_r,eq_ind, eq_sym; reflexivity.
-Defined.
-Next Obligation.
-  unfold noConfusionHom_LE_obligation_1.
-  unfold NoConfusionHom_LE in *.
-  depelim b.
-  - unfold eq_ind_r,eq_ind, eq_sym, LE_n_eq.
-    unfold eq_ind_r,eq_ind,eq_sym,inj_right_pair,f_equal.
-    rewrite eq_dec_refl.
-    unfold K_dec.
-    rewrite <- Eqdep_dec.eq_rect_eq_dec; try reflexivity.
-    + intros x y. left.
-      rewrite Eqdep_dec.UIP_refl_nat with (x := x).
-      rewrite Eqdep_dec.UIP_refl_nat with (x := y).
-      reflexivity.
-  - unfold eq_ind_r,eq_ind, eq_sym; reflexivity.
-Defined.
-
-Equations Derive Subterm for LE.
-
-Lemma LE_eq : forall {n m : nat} (h h' : n ≤ m), h = h'.
-Proof.
-  intros n m h h';
-    induction h; depelim h'.
-  - rewrite LE_n_eq; reflexivity.
-  - exfalso; apply not_S_n_LE_n in h'; inv h'.
-  - clear IHh; exfalso; apply not_S_n_LE_n in h; inv h.
-  - f_equal; auto.
-Defined.
-    
-Equations ext_LE : forall {Δ₁ Δ₂ : nat},
-    (forall n, n ≤ Δ₁ -> n ≤ Δ₂) -> forall {n : nat}, n ≤ S Δ₁ -> n ≤ S Δ₂ :=
-  ext_LE ρ (LE_n _)     := S_LE (ρ _ (LE_n _));
-  ext_LE ρ (LE_S _ _ h) := LE_S _ _ (ρ _ h).
-
-Definition LT (n m : nat) : Set := S n ≤ m.
-Notation "x '`<' y"
-  := (LT x y) (at level 80, no associativity) : type_scope.
-
-Lemma LT_eq : forall {n m : nat} (h h' : n `< m), h = h'.
-Proof.
-  intros n m.
-  refine LE_eq.
-Defined.
-
-Definition S_LT {n m : nat} : n `< m -> S n `< S m := S_LE.
-
-Equations LT_LE : forall {n m : nat}, n `< m -> n ≤ m :=
-  LT_LE (LE_n _)     := LE_S _ _ (LE_n _);
-  LT_LE (LE_S _ _ h) := LE_S _ _ (LT_LE h).
-
-Definition LT_0_l (n : nat) : 0 `< S n := S_LE (LE_0_l n).
-
-Definition S_impl_LT {n m : nat} : S n `< S m -> n `< m := S_impl_LE.
-
-Equations bruh' : forall (m n : nat), (forall r, r `< m -> r `< n) -> m ≤ n :=
-  bruh' 0     n _ := LE_0_l n;
-  bruh' (S m) n ρ := ρ m (LE_n (S m)).
-
-Definition ext_LT {Δ₁ Δ₂ : nat} (ρ : forall n, n `< Δ₁ -> n `< Δ₂)
-  : forall n, n `< S Δ₁ -> n `< S Δ₂.
-Proof.
-  unfold "`<" in *.
-  intros n h. inversion h; subst.
-  - clear h.
-    apply S_LE.
-    auto using bruh'.
-  - constructor.
-    apply ρ, H0.
-Defined.
-
 Inductive type (Δ : nat) : Set :=
-| TId n : n `< Δ -> type Δ
+| TId : Fin.t Δ -> type Δ
 | TForall (τ : type (S Δ)) : type Δ
 | TArrow (τ₁ τ₂ : type Δ) : type Δ.
 
@@ -158,19 +24,19 @@ Equations Derive NoConfusion NoConfusionHom Subterm for type.
 
 Declare Scope ty_scope.
 Delimit Scope ty_scope with ty.
-
+Coercion TId : Fin.t >-> type.
 Notation "'∀' x"
   := (TForall x) (at level 20, right associativity) : ty_scope.
 Notation "x → y"
   := (TArrow x y) (at level 19, right associativity) : ty_scope.
 
 Equations S_type : forall {Δ : nat}, type Δ -> type (S Δ) :=
-  S_type (TId n h)    := TId (S n) (S_LT h);
+  S_type (TId n)      := Fin.FS n;
   S_type (∀ τ)%ty     := (∀ S_type τ)%ty;
   S_type (τ₁ → τ₂)%ty := (S_type τ₁ → S_type τ₂)%ty.
 
 Equations type_eq_dec : forall {Δ : nat} (τ ρ : type Δ), {τ = ρ} + {τ <> ρ} :=
-  type_eq_dec (TId n _) (TId m _) with Nat.eq_dec n m => {
+  type_eq_dec (TId n) (TId m) with Fin.eq_dec n m => {
     | left _     => left _
     | right hneq => right _ };
   type_eq_dec (∀ τ)%ty (∀ ρ)%ty with type_eq_dec τ ρ => {
@@ -182,70 +48,62 @@ Equations type_eq_dec : forall {Δ : nat} (τ ρ : type Δ), {τ = ρ} + {τ <> 
       | right hneq => right _
       | left _     => left _ } };
   type_eq_dec _ _ := right _.
-Next Obligation.
-  f_equal. apply LT_eq.
-Defined.
 
-Equations rename_type : forall {Δ₁ Δ₂ : nat},
-    (forall n, n `< Δ₁ -> n `< Δ₂) -> type Δ₁ -> type Δ₂ :=
-  rename_type ρ (TId _ h)    := TId _ (ρ _ h);
-  rename_type ρ (∀ τ)%ty     := (∀ rename_type (ext_LT ρ) τ)%ty;
-  rename_type ρ (τ₁ → τ₂)%ty := (rename_type ρ τ₁ → rename_type ρ τ₂)%ty.
-
-Definition exts_type : forall {Δ₁ Δ₂ : nat},
-    (forall n, n `< Δ₁ -> type Δ₂) -> forall n, n `< S Δ₁ -> type (S Δ₂).
-Proof.
-  intros Δ₁ Δ₂ σ n h.
-  inversion h; subst.
-  - refine (TId 0 (LT_0_l _)).
-  - refine (rename_type (fun _ => id) (S_type (σ _ H0))).
-Defined.
+Equations exts_type : forall {Δ₁ Δ₂ : nat},
+    (Fin.t Δ₁ -> type Δ₂) -> Fin.t (S Δ₁) -> type (S Δ₂) :=
+  exts_type σ Fin.F1     := Fin.F1;
+  exts_type σ (Fin.FS n) := S_type (σ n).
 
 Equations subs_type : forall {Δ₁ Δ₂ : nat},
-    (forall n, n `< Δ₁ -> type Δ₂) -> type Δ₁ -> type Δ₂ :=
-  subs_type σ (TId _ hn)  := σ _ hn;
-  subs_type σ (τ → τ')%ty := (subs_type σ τ → subs_type σ τ')%ty;
-  subs_type σ (∀ τ)%ty    := (∀ subs_type (exts_type σ) τ)%ty.
-
-Definition S_type_suber : forall {Δ₁ Δ₂ : nat},
-    (forall n, n `< Δ₁ -> type Δ₂) -> forall n, n `< S Δ₁ -> type (S Δ₂).
-Proof.
-  intros Δ₁ Δ₂ f n h.
-  unfold "`<" in *.
-  depelim h.
-  - admit.
-  - eapply S_type, f, h.
-Admitted.
+    (Fin.t Δ₁ -> type Δ₂) -> type Δ₁ -> type Δ₂ :=
+  subs_type σ (TId n)     := σ n;
+  subs_type σ (∀ τ)%ty    := (∀ subs_type (exts_type σ) τ)%ty;
+  subs_type σ (τ → τ')%ty := (subs_type σ τ → subs_type σ τ')%ty.
 
 Lemma S_type_subs : forall {Δ₁ Δ₂ : nat}
-    (σ : forall n, n `< Δ₁ -> type Δ₂) (τ : type Δ₁),
-    S_type (subs_type σ τ) = subs_type (S_type_suber σ) (S_type τ).
+    (σ : Fin.t Δ₁ -> type Δ₂) (τ : type Δ₁),
+    S_type (subs_type σ τ) = subs_type (exts_type σ) (S_type τ).
 Proof.
   intros Δ₁ Δ₂ σ τ.
   funelim (subs_type σ τ).
   - rewrite S_type_equation_1.
     do 2 rewrite subs_type_equation_1.
-    admit. (* maybe use [fin nat]? *)
+    rewrite exts_type_equation_2.
+    reflexivity.
   - rewrite S_type_equation_2.
     do 2 rewrite subs_type_equation_2.
-    rewrite S_type_equation_2.
-    rewrite H. admit. (* lemma for [exts] *)
+    rewrite S_type_equation_2,H. reflexivity.
   - rewrite S_type_equation_3.
     do 2 rewrite subs_type_equation_3.
-    rewrite S_type_equation_3.
-    rewrite H, H0. reflexivity.
-Admitted.
-
-Definition sub_type : forall {Δ : nat}, type (S Δ) -> type Δ -> type Δ.
-Proof.
-  intros Δ body arg.
-  refine (subs_type _ body).
-  clear body. intros n h.
-  inversion h; subst.
-  - apply arg.
-  - clear arg.
-    apply (TId n H0).
+    rewrite S_type_equation_3,H,H0.
+    reflexivity.
 Defined.
+
+Equations sub_type_helper : forall {Δ : nat}, type Δ -> Fin.t (S Δ) -> type Δ :=
+  sub_type_helper τ Fin.F1     := τ;
+  sub_type_helper _ (Fin.FS n) := n.
+
+Require Import Coq.Logic.FunctionalExtensionality.
+
+Lemma exts_sub_type_helper : forall {Δ : nat} (τ : type Δ),
+    exts_type (sub_type_helper τ) = sub_type_helper (S_type τ).
+Proof.
+  intros Δ τ.
+  extensionality body.
+  funelim (exts_type (sub_type_helper τ) body).
+  - rewrite exts_type_equation_1.
+    rewrite sub_type_helper_equation_1.
+    admit.
+  - rewrite exts_type_equation_2.
+    rewrite sub_type_helper_equation_2.
+    funelim (sub_type_helper τ n).
+    + rewrite sub_type_helper_equation_1.
+      admit.
+    + rewrite sub_type_helper_equation_2. reflexivity.
+Abort.
+
+Definition sub_type {Δ : nat} (body : type (S Δ)) (arg : type Δ) : type Δ :=
+  subs_type (sub_type_helper arg) body.
 
 Notation "x '`[[' y ']]'"
   := (sub_type x y) (at level 12, no associativity) : ty_scope.
@@ -253,7 +111,17 @@ Notation "x '`[[' y ']]'"
 Lemma S_type_sub : forall {Δ : nat} (τ : type (S Δ)) (τ' : type Δ),
     S_type (τ `[[ τ' ]])%ty = (S_type τ `[[ S_type τ' ]])%ty.
 Proof.
-Admitted.
+  intros Δ τ τ'. unfold "_ `[[ _ ]]".
+  funelim (subs_type (sub_type_helper τ') τ).
+  - rewrite S_type_equation_1.
+    do 2 rewrite subs_type_equation_1.
+    rewrite sub_type_helper_equation_2.
+    funelim (sub_type_helper τ' n).
+    + rewrite sub_type_helper_equation_1.
+      admit. (* sad. *)
+    + rewrite sub_type_helper_equation_2.
+      reflexivity.
+Abort.
 
 Reserved Notation "Γ '⊢' τ" (at level 80, no associativity).
 
@@ -279,43 +147,6 @@ where "Γ '⊢' τ" := (term Γ τ).
 Derive Signature for term.
 Equations Derive NoConfusion (* NoConfusionHom *) (*Subterm*) for term.
 (*Equations Derive Subterm for term.*)
-
-Definition lookup : forall {Δ : nat} {Γ : list (type Δ)} {n : nat},
-    n `< len Γ -> type Δ.
-Proof.
-  intros Δ Γ.
-  induction Γ as [| τ Γ ih]; cbn; intros [| n] hn.
-  - inv hn.
-  - inv hn.
-  - unfold "`<" in *.
-    depelim hn.
-    + apply τ.
-    + rewrite len_equation_2 in H.
-      injection H as h'. rewrite <- h' in hn.
-      eapply ih,hn.
-  - unfold "`<" in *.
-    eapply ih,S_impl_LE,hn.
-Defined.
-
-Local Transparent len.
-
-Equations lookup' :
-  forall {Δ : nat} {Γ : list (type Δ)} {n : nat}, n `< len Γ -> type Δ :=
-  lookup' (Γ:=τ :: _) (LE_n 1) := τ;
-  lookup' (Γ:=_ :: Γ') (LE_S (S _) _ h) := lookup' (Γ:=Γ') h.
-
-Local Opaque len.
-
-Definition count :
-  forall {Δ : nat} {Γ : list (type Δ)} {n : nat}
-    (h : n `< len Γ), Has (lookup' h) Γ.
-Proof.
-  intros Δ Γ n h.
-  funelim (lookup' h).
-  - left. rewrite lookup'_equation_2. reflexivity.
-  - right. (*Search (lookup' (LE_S (S _) (len _) _)).*)
-    rewrite lookup'_equation_3. apply H.
-Defined.
 
 Declare Scope term_scope.
 Delimit Scope term_scope with term.
@@ -361,8 +192,8 @@ Next Obligation.
   pose proof S_term _ _ _ t as St.
   rewrite S_type_equation_2 in St.
   pose proof (St ⦗ S_type τ ⦘)%term as t'.
-  rewrite S_type_sub. exact t'.
-Defined.
+  admit. (* problem :(. *)
+Abort.
 
 Definition map_has : forall (A B : Set) (f : A -> B) (l : list A) b,
     Has b (map f l) -> {a : A & f a = b & Has a l}.
@@ -411,8 +242,8 @@ Proof.
   intros Δ Γ₁ Γ₂ σ τ h.
   apply map_has in h as [τ' ? h]; subst.
   apply σ in h.
-  apply S_term, h.
-Defined.
+  (*apply S_term, h.*)
+Admitted.
 
 Equations subs : forall {Δ : nat} {Γ₁ Γ₂ : list (type Δ)},
     (forall τ : type Δ, Has τ Γ₁ -> Γ₂ ⊢ τ) ->
